thys/VeriComp/Semantics.thy
@@ -1,7 +1,7 @@
 section \<open>The Dynamic Representation of a Language\<close>
 
 theory Semantics
-  imports Main Behaviour Inf begin
+  imports Main Behaviour Inf Transfer_Extras begin
 
 text \<open>
 The definition of programming languages is separated into two parts: an abstract semantics and a concrete program representation.
@@ -49,25 +49,27 @@ notation
   inf_step ("'(\<rightarrow>\<^sup>\<infinity>')" [] 50) and
   inf_step ("_ \<rightarrow>\<^sup>\<infinity>" [55] 50)
 
-lemma finished_inf: "s \<rightarrow>\<^sup>\<infinity> \<Longrightarrow> \<not> finished step s"
+lemma inf_not_finished: "s \<rightarrow>\<^sup>\<infinity> \<Longrightarrow> \<not> finished step s"
   using inf.cases finished_step by metis
 
 lemma eval_deterministic:
   assumes
-    deterministic: "\<And>x y z. step x y \<Longrightarrow> step x z \<Longrightarrow> y = z"
-  shows "s1 \<rightarrow>\<^sup>* s2 \<Longrightarrow> s1 \<rightarrow>\<^sup>* s3 \<Longrightarrow> finished step s2 \<Longrightarrow> finished step s3 \<Longrightarrow> s2 = s3"
-proof(induction s1 arbitrary: s3 rule: converse_rtranclp_induct)
-  case base
-  then show ?case by (simp add: finished_star)
-next
-  case (step y z)
-  then show ?case
-    by (metis converse_rtranclpE deterministic finished_step)
+    deterministic: "\<And>x y z. step x y \<Longrightarrow> step x z \<Longrightarrow> y = z" and
+    "s1 \<rightarrow>\<^sup>* s2" and "s1 \<rightarrow>\<^sup>* s3" and "finished step s2" and "finished step s3"
+  shows "s2 = s3"
+proof -
+  have "right_unique step"
+    using deterministic by (auto intro: right_uniqueI)
+  with assms show ?thesis
+    by (auto simp: finished_def intro: rtranclp_complete_run_right_unique)
 qed
+
+lemma step_converges_or_diverges: "(\<exists>s'. s \<rightarrow>\<^sup>* s' \<and> finished step s') \<or> s \<rightarrow>\<^sup>\<infinity>"
+  by (smt (verit, del_insts) finished_def inf.coinduct rtranclp.intros(2) rtranclp.rtrancl_refl)
 
 subsection \<open>Behaviour of a dynamic execution\<close>
 
-inductive sem_behaves :: "'state \<Rightarrow> 'state behaviour \<Rightarrow> bool" (infix "\<down>" 50) where
+inductive state_behaves :: "'state \<Rightarrow> 'state behaviour \<Rightarrow> bool" (infix "\<down>" 50) where
   state_terminates:
     "s1 \<rightarrow>\<^sup>* s2 \<Longrightarrow> finished step s2 \<Longrightarrow> final s2 \<Longrightarrow> s1 \<down> (Terminates s2)" |
   state_diverges:
@@ -80,58 +82,60 @@ text \<open>
 Even though the @{term step} transition relation in the @{locale semantics} locale need not be deterministic, if it happens to be, then the behaviour of a program becomes deterministic too.
 \<close>
 
-lemma sem_behaves_deterministic:
+lemma right_unique_state_behaves:
   assumes
-    deterministic: "\<And>x y z. step x y \<Longrightarrow> step x z \<Longrightarrow> y = z"
-  shows "s \<down> b1 \<Longrightarrow> s \<down> b2 \<Longrightarrow> b1 = b2"
-proof (induction s b1 rule: sem_behaves.induct)
-  case (state_terminates s1 s2)
-  show ?case using state_terminates.prems state_terminates.hyps
-  proof (induction s1 b2 rule: sem_behaves.induct)
-    case (state_terminates s1 s3)
-    then show ?case
-      using eval_deterministic deterministic by simp
+    "right_unique (\<rightarrow>)"
+  shows "right_unique (\<down>)"
+proof (rule right_uniqueI)
+  fix s b1 b2
+  assume "s \<down> b1" "s \<down> b2"
+  thus "b1 = b2"
+    by (auto simp: finished_def simp del: not_ex
+        elim!: state_behaves.cases
+        dest: rtranclp_complete_run_right_unique[OF \<open>right_unique (\<rightarrow>)\<close>, of s]
+        dest: final_finished star_inf[OF \<open>right_unique (\<rightarrow>)\<close>, THEN inf_not_finished])
+qed
+
+lemma left_total_state_behaves: "left_total (\<down>)"
+proof (rule left_totalI)
+  fix s
+  show "\<exists>b. s \<down> b"
+    using step_converges_or_diverges[of s]
+  proof (elim disjE exE conjE)
+    fix s'
+    assume "s \<rightarrow>\<^sup>* s'" and "finished (\<rightarrow>) s'"
+    thus "\<exists>b. s \<down> b"
+      by (cases "final s'") (auto intro: state_terminates state_goes_wrong)
   next
-    case (state_diverges s1)
-    then show ?case
-      using deterministic star_inf[THEN finished_inf] by simp
-  next
-    case (state_goes_wrong s1 s3)
-    then show ?case
-      using eval_deterministic deterministic by blast
-  qed
-next
-  case (state_diverges s1)
-  show ?case using state_diverges.prems state_diverges.hyps
-  proof (induction s1 b2 rule: sem_behaves.induct)
-    case (state_terminates s1 s2)
-    then show ?case
-      using deterministic star_inf[THEN finished_inf] by simp
-  next
-    case (state_diverges s1)
-    then show ?case by simp
-  next
-    case (state_goes_wrong s1 s2)
-    then show ?case
-      using deterministic star_inf[THEN finished_inf] by simp
-  qed
-next
-  case (state_goes_wrong s1 s2)
-  show ?case using state_goes_wrong.prems state_goes_wrong.hyps
-  proof (induction s1 b2 rule: sem_behaves.induct)
-    case (state_terminates s1 s3)
-    then show ?case 
-      using eval_deterministic deterministic by blast
-  next
-    case (state_diverges s1)
-    then show ?case
-      using deterministic star_inf[THEN finished_inf] by simp
-  next
-    case (state_goes_wrong s1 s3)
-    then show ?case
-      using eval_deterministic deterministic by simp
+    assume "s \<rightarrow>\<^sup>\<infinity>"
+    thus "\<exists>b. s \<down> b"
+      by (auto intro: state_diverges)
   qed
 qed
+
+subsection \<open>Safe states\<close>
+
+definition safe where
+  "safe s \<longleftrightarrow> (\<forall>s'. step\<^sup>*\<^sup>* s s' \<longrightarrow> final s' \<or> (\<exists>s''. step s' s''))"
+
+lemma final_safeI: "final s \<Longrightarrow> safe s"
+  by (metis final_finished finished_star safe_def)
+
+lemma step_safe: "step s s' \<Longrightarrow> safe s \<Longrightarrow> safe s'"
+  by (simp add: converse_rtranclp_into_rtranclp safe_def)
+
+lemma steps_safe: "step\<^sup>*\<^sup>* s s' \<Longrightarrow> safe s \<Longrightarrow> safe s'"
+  by (meson rtranclp_trans safe_def)
+
+lemma safe_state_behaves_not_wrong:
+  assumes "safe s" and "s \<down> b"
+  shows "\<not> is_wrong b"
+  using \<open>s \<down> b\<close>
+proof (cases rule: state_behaves.cases)
+  case (state_goes_wrong s2)
+  then show ?thesis
+    using \<open>safe s\<close> by (auto simp: safe_def finished_def)
+qed simp_all
 
 end
 
