thys/VeriComp/Transfer_Extras.thy
@@ -1,0 +1,29 @@
+theory Transfer_Extras
+  imports Main
+begin
+
+lemma rtranclp_complete_run_right_unique:
+  fixes R :: "'a \<Rightarrow> 'a \<Rightarrow> bool" and x y z :: 'a
+  assumes "right_unique R"
+  shows "R\<^sup>*\<^sup>* x y \<Longrightarrow> (\<nexists>w. R y w) \<Longrightarrow> R\<^sup>*\<^sup>* x z \<Longrightarrow> (\<nexists>w. R z w) \<Longrightarrow> y = z"
+proof (induction x arbitrary: z rule: converse_rtranclp_induct)
+  case base
+  then show ?case
+    by (auto elim: converse_rtranclpE)
+next
+  case (step x w)
+  hence "R\<^sup>*\<^sup>* w z"
+    using right_uniqueD[OF \<open>right_unique R\<close>]
+    by (metis converse_rtranclpE)
+  with step show ?case
+    by simp
+qed
+
+lemma tranclp_complete_run_right_unique:
+  fixes R :: "'a \<Rightarrow> 'a \<Rightarrow> bool" and x y z :: 'a
+  assumes "right_unique R"
+  shows "R\<^sup>+\<^sup>+ x y \<Longrightarrow> (\<nexists>w. R y w) \<Longrightarrow> R\<^sup>+\<^sup>+ x z \<Longrightarrow> (\<nexists>w. R z w) \<Longrightarrow> y = z"
+  using right_uniqueD[OF \<open>right_unique R\<close>, of x]
+  by (auto dest!: tranclpD intro!: rtranclp_complete_run_right_unique[OF \<open>right_unique R\<close>, of _ y z])
+
+end
